Calculate the second derivative of f(x) = (x^3)/2 + e^x + 4x - 6 from xlsx data in res folder.

To find the second derivative, we first need to find the derivative of the given equation:

dy/dx = (y[i+1] - y[i]) / (x[i+1] - x[i])

We can rewrite this as:

y[i+1] - y[i] = (dy/dx) * (x[i+1] - x[i])

Now, taking the derivative of both sides with respect to x, we get:

d/dx (y[i+1] - y[i]) = d/dx [(dy/dx) * (x[i+1] - x[i])]

Using the product rule of differentiation, we can expand the right-hand side:

d/dx [(dy/dx) * (x[i+1] - x[i])] = (d^2y/dx^2) * (x[i+1] - x[i]) + (dy/dx) * (d/dx) (x[i+1] - x[i])

Since (d/dx) (x[i+1] - x[i]) is equal to 1, we can simplify this to:

d/dx (y[i+1] - y[i]) = (d^2y/dx^2) * (x[i+1] - x[i]) + (dy/dx)

Substituting the expression for dy/dx, we get:

d/dx (y[i+1] - y[i]) = (d^2y/dx^2) * (x[i+1] - x[i]) + (y[i+1] - y[i]) / (x[i+1] - x[i])

Multiplying both sides by (x[i+1] - x[i]), we get:

(d/dx) [(y[i+1] - y[i]) * (x[i+1] - x[i])] = (d^2y/dx^2) * (x[i+1] - x[i])^2 + (y[i+1] - y[i])

Now, we can simplify the left-hand side using the mean value theorem for derivatives:

(d/dx) [(y[i+1] - y[i]) * (x[i+1] - x[i])] = (y[i+2] - 2y[i+1] + y[i]) / (x[i+1] - x[i])^2

Substituting this back into the previous equation, we get:

(y[i+2] - 2y[i+1] + y[i]) / (x[i+1] - x[i])^2 = (d^2y/dx^2) * (x[i+1] - x[i])^2 + (y[i+1] - y[i])

Simplifying, we get:

d^2y/dx^2 = [y[i+2] - 2y[i+1] + y[i]] / [(x[i+1] - x[i])^2]

Therefore, the second derivative of the given equation is:

d^2y/dx^2 = [y[i+2] - 2y[i+1] + y[i]] / [(x[i+1] - x[i])^2]
